src/arch/Arch_s.fst
@@ -1,0 +1,21 @@
+module Arch_s
+
+unfold let nat8_max = 0x100
+unfold let nat16_max = 0x10000
+unfold let nat32_max = 0x100000000
+unfold let nat64_max = 0x10000000000000000
+unfold let nat128_max = 0x100000000000000000000000000000000
+
+// Sanity check our constants
+let _ = assert_norm (pow2 8 = nat8_max)
+let _ = assert_norm (pow2 16 = nat16_max)
+let _ = assert_norm (pow2 32 = nat32_max)
+let _ = assert_norm (pow2 64 = nat64_max)
+let _ = assert_norm (pow2 128 = nat128_max)
+
+type nat8 = x:nat{x < nat8_max}
+type nat16 = x:nat{x < nat16_max}
+type nat32 = x:nat{x < nat32_max}
+type nat64 = x:nat{x < nat64_max}
+type nat128 = x:nat{x < nat128_max}
+
