src/arch/Memory_i_s.fsti
@@ -1,0 +1,165 @@
+module Memory_i_s
+// TODO: eventually, this should be an untrusted module named Memory_i,
+// but we're currently including it in the trusted Semantics_s module(s),
+// so it has to be trusted.
+
+unfold let nat8 = Arch_s.nat8
+unfold let nat16 = Arch_s.nat16
+unfold let nat32 = Arch_s.nat32
+unfold let nat64 = Arch_s.nat64
+
+val heap : Type u#1
+val mem : Type u#1
+
+type base_typ = 
+| TUInt8
+| TUInt16
+| TUInt32
+| TUInt64
+
+type typ =
+| TBase: (b:base_typ) -> typ
+
+let type_of_base_typ (t:base_typ) : Tot Type0 =
+  match t with
+  | TUInt8 -> nat8
+  | TUInt16 -> nat16
+  | TUInt32 -> nat32
+  | TUInt64 -> nat64
+
+let type_of_typ (t:typ) : Tot Type0 =
+  match t with
+  | TBase b -> type_of_base_typ b
+
+val buffer (t:typ) : Type0
+val buffer_as_seq (#t:typ) (h:mem) (b:buffer t) : GTot (Seq.seq (type_of_typ t))
+val buffer_readable (#t:typ) (h:mem) (b:buffer t) : GTot Type0
+val loc : Type u#0
+val loc_none : loc
+val loc_union (s1 s2:loc) : GTot loc
+val loc_buffer (#t:typ) (b:buffer t) : GTot loc
+val loc_disjoint (s1 s2:loc) : GTot Type0
+val loc_includes (s1 s2:loc) : GTot Type0
+val modifies (s:loc) (h1 h2:mem) : GTot Type0
+
+unfold let buffer8 = buffer (TBase TUInt8)
+unfold let buffer16 = buffer (TBase TUInt16)
+unfold let buffer32 = buffer (TBase TUInt32)
+unfold let buffer64 = buffer (TBase TUInt64)
+
+let rec loc_locs_disjoint_rec (l:loc) (ls:list loc) : Type0 =
+  match ls with
+  | [] -> True
+  | h::t -> loc_disjoint l h /\ loc_disjoint h l /\ loc_locs_disjoint_rec l t
+
+let rec locs_disjoint_rec (ls:list loc) : Type0 =
+  match ls with
+  | [] -> True
+  | h::t -> loc_locs_disjoint_rec h t /\ locs_disjoint_rec t
+
+unfold
+let locs_disjoint (ls:list loc) : Type0 = normalize (locs_disjoint_rec ls)
+
+// equivalent to modifies; used to prove modifies clauses via modifies_goal_directed_trans
+val modifies_goal_directed (s:loc) (h1 h2:mem) : GTot Type0
+val lemma_modifies_goal_directed (s:loc) (h1 h2:mem) : Lemma
+  (modifies s h1 h2 == modifies_goal_directed s h1 h2)
+
+val modifies_buffer_elim (#t1:typ) (b:buffer t1) (p:loc) (h h':mem) : Lemma
+  (requires
+    loc_disjoint (loc_buffer b) p /\
+    buffer_readable h b /\
+    modifies p h h'
+  )
+  (ensures
+    buffer_readable h b /\
+    buffer_readable h' b /\
+    buffer_as_seq h b == buffer_as_seq h' b
+  )
+  [SMTPatOr [
+    [SMTPatT (modifies p h h'); SMTPat (buffer_readable h' b)];
+    [SMTPatT (modifies p h h'); SMTPatT (buffer_as_seq h' b)]
+  ]]
+
+val loc_includes_refl (s:loc) : Lemma
+  (loc_includes s s)
+  [SMTPat (loc_includes s s)]
+
+val loc_includes_trans (s1 s2 s3:loc) : Lemma
+  (requires (loc_includes s1 s2 /\ loc_includes s2 s3))
+  (ensures (loc_includes s1 s3))
+
+val loc_includes_union_r (s s1 s2:loc) : Lemma
+  (requires (loc_includes s s1 /\ loc_includes s s2))
+  (ensures (loc_includes s (loc_union s1 s2)))
+  [SMTPat (loc_includes s (loc_union s1 s2))]
+
+val loc_includes_union_l (s1 s2 s:loc) : Lemma
+  (requires (loc_includes s1 s \/ loc_includes s2 s))
+  (ensures (loc_includes (loc_union s1 s2) s))
+  // for efficiency, no SMT pattern
+
+val loc_includes_union_l_buffer (#t:typ) (s1 s2:loc) (b:buffer t) : Lemma
+  (requires (loc_includes s1 (loc_buffer b) \/ loc_includes s2 (loc_buffer b)))
+  (ensures (loc_includes (loc_union s1 s2) (loc_buffer b)))
+  [SMTPat (loc_includes (loc_union s1 s2) (loc_buffer b))]
+
+val loc_includes_none (s:loc) : Lemma
+  (loc_includes s loc_none)
+  [SMTPat (loc_includes s loc_none)]
+
+val modifies_refl (s:loc) (h:mem) : Lemma
+  (modifies s h h)
+  [SMTPat (modifies s h h)]
+
+val modifies_goal_directed_refl (s:loc) (h:mem) : Lemma
+  (modifies_goal_directed s h h)
+  [SMTPat (modifies_goal_directed s h h)]
+
+val modifies_loc_includes (s1:loc) (h h':mem) (s2:loc) : Lemma
+  (requires (modifies s2 h h' /\ loc_includes s1 s2))
+  (ensures (modifies s1 h h'))
+  // for efficiency, no SMT pattern
+
+val modifies_trans (s12:loc) (h1 h2:mem) (s23:loc) (h3:mem) : Lemma
+  (requires (modifies s12 h1 h2 /\ modifies s23 h2 h3))
+  (ensures (modifies (loc_union s12 s23) h1 h3))
+  // for efficiency, no SMT pattern
+
+// Prove (modifies s13 h1 h3).
+// To avoid unnecessary matches, don't introduce any other modifies terms.
+// Introduce modifies_goal_directed instead.
+val modifies_goal_directed_trans (s12:loc) (h1 h2:mem) (s13:loc) (h3:mem) : Lemma
+  (requires
+    modifies s12 h1 h2 /\
+    modifies_goal_directed s13 h2 h3 /\
+    loc_includes s13 s12
+  )
+  (ensures (modifies s13 h1 h3))
+  [SMTPat (modifies s12 h1 h2); SMTPat (modifies s13 h1 h3)]
+
+val modifies_goal_directed_trans2 (s12:loc) (h1 h2:mem) (s13:loc) (h3:mem) : Lemma
+  (requires
+    modifies s12 h1 h2 /\
+    modifies_goal_directed s13 h2 h3 /\
+    loc_includes s13 s12
+  )
+  (ensures (modifies_goal_directed s13 h1 h3))
+  [SMTPat (modifies s12 h1 h2); SMTPat (modifies_goal_directed s13 h1 h3)]
+
+val buffer_read (#t:typ) (b:buffer t) (i:int) (h:mem) : Pure (type_of_typ t)
+  (requires True)
+  (ensures (fun v ->
+    0 <= i /\ i < Seq.length (buffer_as_seq h b) /\ buffer_readable h b ==>
+    v == Seq.index (buffer_as_seq h b) i
+  ))
+
+val buffer_write (#t:typ) (b:buffer t) (i:int) (v:type_of_typ t) (h:mem) : Pure mem
+  (requires True)
+  (ensures (fun h' ->
+    0 <= i /\ i < Seq.length (buffer_as_seq h b) /\ buffer_readable h b ==>
+    modifies (loc_buffer b) h h' /\
+    buffer_readable h' b /\
+    buffer_as_seq h' b == Seq.upd (buffer_as_seq h b) i v
+  ))
+
