src/arch/x64/X64.Vale.StateLemmas_i.fsti
@@ -22,14 +22,10 @@ val lemma_to_flags : s:state -> Lemma
   (ensures s.flags == UInt64.v (flags' (state_to_S s)))
   [SMTPat s.flags]
 
-val lemma_to_mem_contains : s:state -> i:int -> Lemma
-  (ensures Map.contains s.mem i = Map.contains (mem' (state_to_S s)) i)
-  [SMTPat (Map.contains s.mem i)]
+val lemma_to_mem : s:state -> Lemma
+  (ensures s.mem == mem' (state_to_S s))
+  [SMTPat s.mem]
   
-val lemma_to_mem_sel : s:state -> i:int -> Lemma
-  (ensures Map.sel s.mem i == UInt64.v (Map.sel (mem' (state_to_S s)) i))
-  [SMTPat (Map.sel s.mem i)]
-
 val lemma_to_reg : s:state -> r:reg -> Lemma
   (ensures s.regs r == UInt64.v (regs' (state_to_S s) r))
   [SMTPat (s.regs r)]
